\documentclass[11pt]{article}
\usepackage{amsfonts}
\usepackage{amsmath}
\usepackage{graphicx}
\usepackage[normalem]{ulem}
\usepackage[a4paper, total={6in, 8in}]{geometry}
\usepackage{listings}
\usepackage{amssymb}
\usepackage{color} %red, green, blue, yellow, cyan, magenta, black, white
\definecolor{mygreen}{RGB}{28,172,0} % color values Red, Green, Blue
\definecolor{mylilas}{RGB}{170,55,241}
\def\ny{\mathcal N \bold y}
\def\nx{\mathcal N \bold x}
\def\bx{\bold x}
\def\by{\bold y}
\def\tx{T \bold x}
\def\ty{T \bold y}
\newcommand\norm[1]{\left\lVert#1\right\rVert}
\newcommand\vc[1]{\left\langle{#1}\right\rangle }
\newcommand*{\QEDA}{\hfill\ensuremath{\blacksquare}}
\newcommand\bra[1]{\left( #1 \right)}
\def \xy{\norm{\bx - \by}^2}
\def \nxny{\norm{\nx  - \ny}^2}
\def \txty{\norm{\tx  - \ty}^2}
\def \tt{\tx - \ty}
\def \xx{\bx - \by}
\def \pr{\operatorname{prox}_{\|\cdot\|_{1}}}
\def \px{\pr \bx}
\def \py{\pr \by}

\title{\textbf{Mathematical Modeling HW5}}
\author{\textsc{Miyasaka} Kion}
\date{\today}

\begin{document}	
\maketitle

\lstset{language=Matlab,%
    %basicstyle=\color{red},
    breaklines=true,%
    morekeywords={matlab2tikz},
    keywordstyle=\color{blue},%
    morekeywords=[2]{1}, keywordstyle=[2]{\color{black}},
    identifierstyle=\color{black},%
    stringstyle=\color{mylilas},
    commentstyle=\color{mygreen},%
    showstringspaces=false,%without this there will be a symbol in the places where there is a space
    numbers=left,%
    numberstyle={\tiny \color{black}},% size of the numbers
    numbersep=9pt, % this defines how far the numbers are from the text
    emph=[1]{for,end,break},emphstyle=[1]\color{red}, %some words to emphasise
    %emph=[2]{word1,word2}, emphstyle=[2]{style},    
}

\section{Task: Prove proposition 4.1}
Proposition 4.1. The following are equivalent:

(i) $T$ is firmly nonexpansive.

(ii) $T$ is $\frac{1}{2}$-averaged nonexpansive.

(iii) $\mathcal{I}-T$ is firmly nonexpansive.

(iv) $2 T-\mathcal{I}$ is nonexpansive.
\paragraph{Proof$_1$} We first prove (ii) and (i) are equivalent, i.e.  $T$ is $\frac{1}{2}$-averaged nonexpansive if and only if $T$ is firmly nonexpansive. $T$ is $\frac{1}{2}$-averaged nonexpansive which means $T$ can be written as $\frac{\mathcal I + \mathcal N}{2}$, where $\mathcal N$ is a non-expansive operator:
$$
\norm{ \mathcal N \bold x + \mathcal N \bold y }  \leq \norm{ \bold x - \bold y } \iff \norm{ \mathcal N \bold x + \mathcal N \bold y } ^2 \leq \norm {\bold x - \bold y }^2
$$
add some components to construct the inequality above, we have
$$
\begin{aligned}
	\| \bold x - \bold y \|^2 + 2 \langle \bold x - \bold y, \mathcal N \bold x - \mathcal N \bold y \rangle +  \| \mathcal N \bold x + \mathcal N \bold y \| ^2 
&\leq
2  \| \bold x - \bold y \|^2 + 2 \langle \bold x - \bold y, \mathcal N \bold x - \mathcal N \bold y \rangle
\end{aligned}
$$
where
$$
\begin{aligned}
	\text{LHS} &= \langle (\bold x - \bold y) + (\mathcal N \bold x - \mathcal N \bold y), (\bold x - \bold y) + (\mathcal N \bold x - \mathcal N \bold y) \rangle \\
	&= \norm{ \bx - \by + \nx - \ny} \\
	\text{RHS}&= 2 \langle \bold x - \bold y, \bold x - \bold y\rangle  + 2 \langle \bold x - \bold y , \nx  - \mathcal N \bold y\rangle \\
	&= 2 \langle \bx - \by  + \nx - \ny ,\bx - \by \rangle
\end{aligned}
$$
Since LHS $\leq$ RHS, we have 
$$
\norm{\frac {\bx + \nx}{2} - \frac{\by + \ny}{2}} ^ 2 \leq \vc{\frac{\bx + \nx}{2} - \frac{\by + \ny}{2},\bx - \by}
$$
which is equivalent to 
$$
\norm{\tx - \ty }^2 \leq \norm{\bx - \by}.
$$.
 \QEDA
\paragraph{Proof$_2$} Now we prove (iii) and (ii) are equivalent, i.e. $\mathcal I- T$ is firmly nonexpansive if and only if   $T$ is $\frac{1}{2}$-averaged nonexpansive.  $\mathcal I- T$  is firmly nonexpansive infers
$$
\norm{(\bx - \tx) - (\by - \ty)} ^ 2 \leq \vc{(\bx - \tx) - (\by - \ty), \bx - \by}
$$
let $\mathcal N$ such that that $T = \frac{\mathcal I + \mathcal N }{2}$, we have
$$
\begin{aligned}
	\text{LHS}&=\norm{\bra{\bx - \frac{\bx + \nx}{2} } - \bra{\by - \frac{\by + \ny}{2}}}^2\\
	&= 1/4 \cdot \norm {\bx - \by - \bra{\nx - \ny}}\\
	\text{RHS}&= 1/2 \cdot \vc{\bx - \by - \bra {\nx - \ny},\bx - \by}
\end{aligned}
$$
Then,
$$
 \begin{aligned}
 	&\norm {\bx - \by - \bra{\nx - \ny}}^2  \leq  2 \vc{\bx - \by - \bra {\nx - \ny},\bx - \by} \\
 	&\iff  \\
 	 &\norm{\bx - \by}^2  + \norm{\nx - \ny}^2  - 2 \vc{\bx - \by - \bra {\nx - \ny},\bx - \by} \leq  2 \vc{\bx - \by}^2 - 2 \vc{\bx - \by - \bra {\nx - \ny},\bx - \by} \\
 	& \iff \\
 	& \norm{\nx - \ny}^2 \leq  \xy 
 \end{aligned}
$$
If  $\mathcal I- T$ is firmly nonexpansive, we can assume that $\mathcal N$ does not exist, the above inequality cannot satisfied, i.e. there exist a nonexpansive operator $\mathcal N$ s.t.  $T = \frac{\mathcal I + \mathcal N }{2}$. If  $T$ is $\frac{1}{2}$-averaged nonexpansive, then let $\mathcal N$ be a nonexpasive operator s.t. $T = \frac{\mathcal I + \mathcal N }{2}$, we can infer that  $\mathcal I- T$ is firmly nonexpansive,

\QEDA
\paragraph{Proof$_3$} Finally we prove (i) and (iv) are equivalent, i.e. $2 T-\mathcal{I}$ is nonexpansive if and only if  $T$ is firmly nonexpansive. $2 T-\mathcal{I}$ is nonexpansive means 
$$
\begin{aligned}
	\norm{\bra{2\tx  - \bx}- \bra {2\ty  - \by}} &\leq  \norm{\bx - \by}\\
	\iff \norm{2\bra{\tx - \ty} - \bra{\bx - \by}}^2 &\leq \xy\\
	\iff 4 \txty  + \xy- 4 \vc{\tt,\xx} &\leq \xy \\
	\iff \txty &\leq \xy \\
	\iff \norm{\tt} &\leq \norm{\bx - \by}\quad \text{($T$ is nonexpansive)}
\end{aligned}
$$
\QEDA

\section{Task: $\operatorname{prox}_{\|\cdot\|_{1}}$ is firmly nonexpansive}  Prove that $\operatorname{prox}_{\|\cdot\|_{1}}$ is firmly nonexpansive according to (3.7) and (3.8). (Don't use Theorem 4.1 !!!)
\begin{itemize}
	\item One-dimensional case
For $x \in \mathbb{R}$,
$$
\operatorname{prox}_{|\cdot|}(x)=\max \{|x|-1,0\} \cdot \operatorname{sgn}(x)
$$
\item $n$-dimensional case
For $\boldsymbol{x} \in \mathbb{R}^{n}$,
$$
\operatorname{prox}_{\|\cdot\|_{1}}(\boldsymbol{x})=\left(\operatorname{prox}_{|\cdot|}\left(x_{1}\right), \operatorname{prox}_{|\cdot|}\left(x_{2}\right), \ldots, \operatorname{prox}_{|\cdot|}\left(x_{n}\right)\right)^{\top}
$$
\end{itemize}

\paragraph{Proof} We prove by mathematical induction.
\subparagraph{Base case: 1-dimension case}
$\pr$ is defined by
$$
\pr (x) = \max \{|x|-1,0\} \cdot \operatorname{sgn}(x)
$$
We hope $\pr$ is firmly nonexpansive i.e. we hope that
$$
\begin{aligned}
	\norm{\pr \bx - \pr \by}^2 \leq \vc{\ \pr \bx - \pr \by,\bx - \by} \\
\iff \vc{\pr \bx - \pr \by , \pr \bx - \pr \by - (\bx - \by ) }\leq 0
\end{aligned}
$$
We expand the LHS above,
$$
\begin{aligned}
	&\text{LHS} \\
	&= (\text{sgn}(x) \max (0,| x| -1)-\text{sgn}(y) \max (0,| y| -1)) (\text{sgn}(x) \max (0,| x| -1)-\text{sgn}(y) \max (0,| y| -1)-x-y) \\
	&=\begin{cases}
		 (| x| -1) \text{sgn}(x) ((| x| -1) \text{sgn}(x)-x+y) & | x| >1\land | y| \leq 1 \\
 ((| x| -1) \text{sgn}(x)-(| y| -1) \text{sgn}(y)) ((| x| -1) \text{sgn}(x)-| y|  \text{sgn}(y)+\text{sgn}(y)-x+y) & | x| >1\land | y| >1 \\
 (| y| -1) \text{sgn}(y) ((| y| -1) \text{sgn}(y)+x-y) & | x| \leq 1\land | y| >1 \\
	\end{cases}
 \\
 &\leq 0 \quad \text{(Since the maximum of all cases are less or equal than 0 ).}
\end{aligned}
$$



Therefore, $\pr$ is a firmly nonexpansive when dimension is 1.

\subparagraph{Induction step}
if $\pr$ is firmly nonexpensive when $\bx \in \mathbb R^n$, i.e. by definition of $\pr$, we have
$$
\norm{\px - \py}^2 \leq \vc{\px - \py, \bx - \by}
$$
which is equivalent to 
$$
\sum_{i=1}^{n}\bra{\pr x_i - \pr y_i}^2 \leq \sum_{i=1}^{n}\bra{\pr x_i - \pr y_i}\cdot \bra{x_i - y_i}
$$
for $\pr$ is firmly nonexpansive when dimension is 1, 
$$
\bra{\pr x_{n+1} - \pr y_{n+1} }^2 \leq\bra{\pr x_{n+1} - \pr y_{n+1}}\bra{x_{n+1} - y_{n+1}}
$$
by adding the 2 inequality above we get 
$$
\sum_{i=1}^{n+1}\bra{\pr x_i - \pr y_i}^2 \leq \sum_{i=1}^{n+1}\bra{\pr x_i - \pr y_i}\cdot \bra{x_i - y_i}
$$
which infers that $\norm{\px - \py}^2 \leq \vc{\px - \py, \bx - \by}$ holds when $\bx \in \mathbb R^{n+1}$.

Hence $\pr$ is firmly nonexpansive.

\QEDA
\end{document}